src/Init/Data/List/Basic.lean
@@ -900,7 +900,7 @@ theorem mem_of_elem_eq_true [BEq α] [LawfulBEq α] {a : α} {as : List α} : el
     next h => intros; simp [BEq.beq] at h; subst h; apply Mem.head
     next _ => intro h; exact Mem.tail _ (mem_of_elem_eq_true h)
 
-theorem elem_eq_true_of_mem [BEq α] [LawfulBEq α] {a : α} {as : List α} (h : a ∈ as) : elem a as = true := by
+theorem elem_eq_true_of_mem [BEq α] [ReflBEq α] {a : α} {as : List α} (h : a ∈ as) : elem a as = true := by
   induction h with
   | head _ => simp [elem]
   | tail _ _ ih => simp [elem]; split; rfl; assumption
